\documentclass[11pt,compress,t,notes=noshow, xcolor=table]{beamer}
\input{../../style/preamble}
\input{../../latex-math/basic-math}
\input{../../latex-math/basic-ml}

\title{Introduction to Machine Learning}

\begin{document}
    
\titlemeta{% Chunk title (example: CART, Forests, Boosting, ...), can be empty
    Information Theory
  }{% Lecture title  
    Entropy II
  }{% Relative path to title page image: Can be empty but must not start with slides/
  figure/entropy_bernoulli.png
  }{
  \item Further properties of entropy and joint entropy
  \item Understand that uniqueness theorem justifies choice of entropy formula
  \item Maximum entropy principle
}

\begin{vbframe}{Entropy of Bernoulli distribution}

Let $X$ be Bernoulli / a coin with $\P(X=1) = s$ and $\P(X=0) = 1 - s$.

$$ H(X)= -s \cdot \log_2(s)-(1-s)\cdot \log_2(1-s). $$

\begin{center}
\includegraphics[width = 8.0cm ]{figure/entropy_bernoulli.png} \\
\end{center}

We note: If the coin is deterministic, so $s=1$ or $s=0$, then $H(s)=0$; 
$H(s)$ is maximal for $s = 0.5$, a fair coin. 
$H(s)$ increases monotonically the closer we get to $s=0.5$.
This all seems plausible.

\end{vbframe}

\begin{vbframe} {Joint entropy}
\begin{itemize}
  \item The \textbf{joint entropy} of two discrete random variables $X$ and $Y$ is:
    $$ H(X,Y) = H(p_{X,Y}) = - \sum_{x \in \Xspace} \sum_{y \in \Yspace}  p(x,y) \log_2(p(x,y))$$
  % where $I(x,y)$ is the self-information of $(x,y)$.
  \item Intuitively, the joint entropy is a measure of the total uncertainty in the two variables $X$ and $Y$. In other words, it is simply the entropy of the joint distribution $p(x,y)$.
  \item There is nothing really new in this definition because $H(X, Y)$ can be considered to be a single vector-valued random variable.
  \item More generally:
    \begin{footnotesize}  
  $$ H(X_1, X_2, \ldots, X_n) = - \sum_{x_1 \in \Xspace_1} \ldots \sum_{x_n \in \Xspace_n} p(x_1,x_2, \ldots, x_n) \log_2(p(x_1,x_2, \ldots, x_n)) $$ 
    \end{footnotesize}  
\end{itemize}
\end{vbframe}

\begin{vbframe} {Entropy is additive under independence}
\begin{enumerate}
\setcounter{enumi}{6}
    \item Entropy is additive for independent RVs.
\end{enumerate}
\vspace{0.2cm}
Let $X$ and $Y$ be two independent RVs. Then:
  \begin{small}
  \begin{equation*}
    \begin{aligned} 
     H(X,Y) &= - \sum_{x \in \Xspace} \sum_{y \in \Yspace}  p(x,y) \log_2(p(x,y)) \\ 
            &= - \sum_{x \in \Xspace} \sum_{y \in \Yspace}  p_X(x)p_Y(y) \log_2(p_X(x)p_Y(y)) \\
            &= - \sum_{x \in \Xspace} \sum_{y \in \Yspace}  p_X(x)p_Y(y)\log_2(p_X(x)) + p_X(x)p_Y(y)\log_2(p_Y(y)) \\
            &= - \sum_{x \in \Xspace} \sum_{y \in \Yspace}  p_X(x)p_Y(y)\log_2(p_X(x)) - \sum_{y \in \Yspace} \sum_{x \in \Xspace} p_X(x)p_Y(y)\log_2(p_Y(y)) \\
            &= - \sum_{x \in \Xspace} p_X(x)\log_2(p_X(x)) - \sum_{y \in \Yspace} p_Y(y)\log_2(p_Y(y)) = H(X) + H(Y)
    \end{aligned} 
  \end{equation*}
\end{small}
% \begin{itemize}
% \end{itemize}
\end{vbframe}



\begin{vbframe}{The Uniqueness Theorem}

\citelink{KHINCHIN1957MATHEMATICAL} showed that the only family of functions satisfying
\begin{itemize}
  \item $H(p)$ is continuous in probabilities $p(x)$
  \item adding or removing an event with $p(x)=0$ does not change it
  \item is additive for independent RVs
  \item is maximal for a uniform distribution.
\end{itemize}

is of the following form:

$$ H(p) = - \lambda \sum_{x \in \Xspace} p(x) \log p(x) $$ 

where $\lambda$ is a positive constant. Setting $\lambda = 1$ and using the binary logarithm gives us the Shannon entropy.
\end{vbframe}

\begin{vbframe}{The Maximum Entropy Principle}

Assume we know $M$ properties about a discrete distribution $p(x)$ on $\Xspace$, stated as ``moment conditions'' for functions $g_m(\cdot)$ and scalars $\alpha_m$:
\normalsize{$$\mathbb{E}[g_m(X)]=\sum_{x \in \Xspace}g_m(x)p(x) = \alpha_m\,\,\text{for}\,\, m=0,\ldots,M$$}
\vspace{-0.4cm}

\textbf{Maximum entropy principle} \citelink{JAYNES_2003}: Among all feasible distributions satisfying the constraints, choose the one with maximum entropy!
\begin{itemize}
    \item Motivation: ensure no unwarranted assumptions on $p(x)$ are made beyond what we know. 
    \item MEP follows similar logic to Occam's razor and principle of insufficient reason
\end{itemize}


\end{vbframe}

\begin{vbframe}{The Maximum Entropy Principle}
Can be solved via Lagrangian multipliers (here with base $e$)
\small{$$L(p(x),(\lambda_m)_{m=0}^{M}) = - \sum_{x \in \Xspace} p(x) \log(p(x)) + \lambda_0 \big( \sum_{x \in \Xspace} p(x) - 1 \big) + \sum_{m=1}^{M} \lambda_m \big( \sum_{x \in \Xspace} g_m(x)p(x)-\alpha_m \big)$$}
Finding critical points $p^{\ast}(x)$ :
$$\frac{\partial L}{\partial p(x)} = -\log(p(x)) -1 + \lambda_0 + \sum_{m=1}^{M} \lambda_m g_m(x) \overset{!}{=} 0 \iff p^{\ast}(x)=\textcolor{blue}{\exp(\lambda_0-1)}\textcolor{red}{
\exp\big(\sum_{m=1}^{M} \lambda_m g_m(x)\big)}$$
This is a maximum as $-1/p(x)<0$. Since probs must sum to 1 we get
$$1\overset{!}{=}\sum_{x \in \Xspace} p^{\ast}(x)=\textcolor{blue}{\frac{1}{\exp(1-\lambda_0)}} \sum_{x \in \Xspace} \textcolor{red}{\exp\big(\sum_{m=1}^{M} \lambda_m g_m(x)\big)} \Rightarrow \textcolor{blue}{\exp(1-\lambda_0)}=\textcolor{blue}{\sum_{x \in \Xspace} \exp\big(\sum_{m=1}^{M} \lambda_m g_m(x)\big)}$$
Plugging $\textcolor{blue}{\exp(1-\lambda_0)}$ into $p^{\ast}(x)$ we obtain the constrained maxent distribution:

$$p^{\ast}(x)=\frac{\textcolor{red}{\exp{\sum_{m=1}^{M}\lambda_m g_m(x)}}}{\textcolor{blue}{\sum_{x \in \Xspace} \exp{\sum_{m=1}^{M}\lambda_m g_m(x)}}}$$

\end{vbframe}

\begin{vbframe}{The Maximum Entropy Principle}

We now have: functional form of our distribution, up to $M$ unknowns, the $\lambda_m$. But also: $M$ equations, the moment conditions. So we can solve.

\vspace{0.5cm}

\textbf{Example}: Consider discrete RV representing a six-sided die roll and the moment condition $\mathbb{E}(X)=4.8$. What is the maxent distribution?\\

\begin{itemize}
\setlength{\itemsep}{0.9em}
    \item Condition means $g_1(x)=x$, $\alpha_1=4.8$. Then for some $\lambda$ solution is
    {\small $$p^{\ast}(x)=\frac{\exp{(\lambda g(x))}}{\sum_{j=1}^{6} \exp({\lambda g(x_j)})} = \frac{\exp{(\lambda x)}}{\sum_{j=1}^{6} \exp{(\lambda x_j)}}$$}
    \item Inserting into moment condition and solving (numerically) for $\lambda$: 
    $$4.8\overset{!}{=}\sum_{j=1}^{6} x_j p^{\ast}(x_j) = \frac{e^\lambda+\ldots+6(e^\lambda)^6}{e^\lambda+\ldots+(e^{\lambda})^6} \Rightarrow \lambda \approx 0.5141$$
{\small
\begin{tabular}{|c|c|c|c|c|c|c|c}
\hline
x & 1 & 2 & 3 & 4 & 5 & 6 \\ 
\hline
$p^{\ast}(x)$ & 3.22\% & 5.38\% & 9.01\% & 15.06\% & 25.19\% & 42.13\%\\ 
\hline
\end{tabular}
}
%\item For a fair die ($\mathbb{E}(X)=\alpha_1=3.5$) it is not hard to see that $\lambda=0$ satisfies the equation, resulting in uniform probabilities
\end{itemize}
\end{vbframe}



\endlecture
\end{document}

